overall structure termin done

wip/formalization/Termination.v
@@ -1,1 +1,52 @@
 Require Export SigmaMatch.
+Require Import Init.Wf.
+
+
+
+
+Definition Triple_order (Q Q': nat * nat * nat) :=
+  let N1  := fst (fst Q) in
+  let N1' := fst (fst Q') in
+  let N2  := snd (fst Q) in
+  let N2' := snd (fst Q') in
+  let N3  := snd Q in
+  let N3' := snd Q' in
+   (N1 > N1') \/
+  ((N1 >= N1') /\ (N2 > N2')) \/
+  (((N1 >= N1') /\ (N2 >= N2')) /\ (N3 > N3')).
+
+
+Definition Problem_measure (P: Problem) :=
+  (length (Problem_vars P), Problem_size P, σmin_steps_possible P).
+
+
+Definition smatch_step_size_order (T T' : Tuple) := 
+  Triple_order (Problem_measure (snd T')) (Problem_measure (snd T)).
+
+
+Definition smatch_step_order (T T' : Tuple) :=  smatch T' T.
+
+Notation "T <<* T'" := (smatch_step_size_order T T') (at level 67).
+
+
+Lemma smatch_step_termination : forall T T',  smatch T T' ->  T' <<* T.
+Admitted.
+
+
+
+(* This is standard because lexicographic ordering of triples of natural numbers is obviously well-founded *)
+Lemma smatch_step_size_order_wf : well_founded smatch_step_size_order.
+Admitted.
+
+
+
+Lemma unif_step_order_wf : well_founded smatch_step_order.
+Proof.
+  unfold well_founded. intro T.
+  apply well_founded_ind with (R:= smatch_step_size_order).
+  apply smatch_step_size_order_wf. intros T' H.
+  apply Acc_intro. intros T'' H0.
+  unfold smatch_step_order in H0.
+  apply smatch_step_termination in H0.
+  apply H; trivial.
+Qed.
